thy/Conc_Impl.thy
@@ -1,6 +1,7 @@
 section{*Imparative implementation*}
 theory Conc_Impl
 imports PointerMapImpl AbstractInterpretation
+  "$AFP/Automatic_Refinement/Lib/Refine_Lib"
 begin
 
 instantiation prod :: (default, default) default
@@ -29,29 +30,60 @@ definition destrci :: "nat \<Rightarrow> (nat \<times> nat \<times> nat) pointer
 	Suc 0 \<Rightarrow> return TD |
 	Suc (Suc p) \<Rightarrow> pm_pthi bdd p \<guillemotright>= (\<lambda>(v,t,e). return (IFD v t e)))"
 
-lemma [sep_heap_rules]: "<is_pointermap_impl bdd bddi> tci bddi <\<lambda>r. is_pointermap_impl bdd (snd r) * \<up>(fst r = fst (tmi bdd))>"
-by(sep_auto simp: tci_def)
-lemma [sep_heap_rules]: "<is_pointermap_impl bdd bddi> fci bddi <\<lambda>r. is_pointermap_impl bdd (snd r) * \<up>(fst r = fst (fmi bdd))>"
-by(sep_auto simp: fci_def)
-lemma [sep_heap_rules]: "(p, u) = ifmi v t e bdd \<Longrightarrow>
-	<is_pointermap_impl bdd bddi> ifci v t e bddi
-	<\<lambda>(pi,ui). is_pointermap_impl u ui * \<up>(pi = p)>\<^sub>t"
-by(sep_auto simp: ifci_def apfst_def map_prod_def split: prod.splits if_splits)
+lemma "(42,1)\<in>{(v,v). v=1}" by simp
+
+definition "node_rel bdd \<equiv> {(v,v) | v. bdd_node_valid bdd v}"
+
+lemma [sep_heap_rules]: "tmi bdd = (p,bdd') 
+  \<Longrightarrow> <is_pointermap_impl bdd bddi> 
+        tci bddi 
+      <\<lambda>(pi,bddi'). is_pointermap_impl bdd' bddi' * \<up>((pi,p)\<in>node_rel bdd')>"
+by(sep_auto simp: tci_def node_rel_def bdd_node_valid_def)
+
+lemma [sep_heap_rules]: "fmi bdd = (p,bdd') 
+  \<Longrightarrow> <is_pointermap_impl bdd bddi> 
+        fci bddi 
+      <\<lambda>(pi,bddi'). is_pointermap_impl bdd' bddi' * \<up>((pi,p)\<in>node_rel bdd')>"
+by(sep_auto simp: fci_def node_rel_def bdd_node_valid_def)
+
+lemma [sep_heap_rules]: "\<lbrakk>(p, bdd') = ifmi v t e bdd; (ti,t)\<in>node_rel bdd; (ei,e)\<in>node_rel bdd \<rbrakk> \<Longrightarrow>
+	<is_pointermap_impl bdd bddi> ifci v ti ei bddi
+	<\<lambda>(pi,bddi'). is_pointermap_impl bdd' bddi' * \<up>((pi,p)\<in>node_rel bdd')>\<^sub>t"
+by(sep_auto 
+  simp: ifci_def apfst_def map_prod_def node_rel_def bdd_node_valid_def
+  split: prod.splits if_splits)
+
 lemma [sep_heap_rules]: "
 	bdd_node_valid bdd n \<Longrightarrow>
 	<is_pointermap_impl bdd bddi> destrci n bddi
 	<\<lambda>r. is_pointermap_impl bdd bddi * \<up>(r = destrmi n bdd)>"
 by(cases "(n, bdd)" rule: destrmi.cases) (sep_auto simp: destrci_def bdd_node_valid_def)+
 
+lemma [simp]: 
+  "bdd_node_valid bdd 0"
+  "bdd_node_valid bdd (Suc 0)"
+  by (auto simp: bdd_node_valid_def)
+
+lemma bdd_node_valid_RmiI: "(ni,n)\<in>Rmi bdd \<Longrightarrow> bdd_node_valid bdd ni"
+  apply (auto simp: Rmi_def)
+  apply (cases "(ni,n,bdd)" rule: Rmi_g.cases; simp)
+  apply (auto simp: bdd_node_valid_def)
+  done
+
 definition "restrict_topci p var val bdd = do {
 	d \<leftarrow> destrci p bdd;
 	return (case d of IFD v t e \<Rightarrow> (if v = var then (if val then t else e) else p) | _ \<Rightarrow> p)
 }"
+
+thm brofix.restrict_top_R[THEN bdd_node_valid_RmiI]
+
 lemma [sep_heap_rules]: "
 	bdd_node_valid bdd p \<Longrightarrow>
 	<is_pointermap_impl bdd bddi> restrict_topci p var val bddi
-	<\<lambda>r. is_pointermap_impl bdd bddi * \<up>(r = brofix.restrict_top_impl p var val bdd)>"
-by(sep_auto simp: restrict_topci_def)
+	<\<lambda>r. is_pointermap_impl bdd bddi * \<up>((r, brofix.restrict_top_impl p var val bdd) \<in> node_rel bdd)>"
+	unfolding node_rel_def apply (simp del: brofix.restrict_top_impl.simps)
+
+  by(sep_auto simp: restrict_topci_def)
 
 fun lowest_topsci where
 "lowest_topsci [] s = return None" |
@@ -70,6 +102,69 @@ lemma [sep_heap_rules]: "
 	<is_pointermap_impl bdd bddi> lowest_topsci es bddi
 	<\<lambda>r. is_pointermap_impl bdd bddi * \<up>(r = brofix.lowest_tops_impl es bdd)>"
 by(induction es) (sep_auto simp:)+
+
+
+partial_function(heap) iteci where
+"iteci i t e s = do {
+  lt \<leftarrow> lowest_topsci [i, t, e] s;
+  case lt of
+		Some a \<Rightarrow> do {
+			ti \<leftarrow> restrict_topci i a True s;
+			tt \<leftarrow> restrict_topci t a True s;
+			te \<leftarrow> restrict_topci e a True s;
+			fi \<leftarrow> restrict_topci i a False s;
+			ft \<leftarrow> restrict_topci t a False s;
+			fe \<leftarrow> restrict_topci e a False s;
+			(tb,s) \<leftarrow> iteci ti tt te s;
+			(fb,s) \<leftarrow> iteci fi ft fe s;
+      (ifci a tb fb s)
+     } 
+  | None \<Rightarrow> do {
+    d \<leftarrow> destrci i s;
+    case d of
+      TD \<Rightarrow> return (t,s)
+    | FD \<Rightarrow> return (e,s)
+   }
+  }"
+
+lemma "(brofix.ite_impl i t e bdd = Some (p,bdd') 
+  \<and> bdd_node_valid bdd i
+  \<and> bdd_node_valid bdd t
+  \<and> bdd_node_valid bdd e
+  ) \<longrightarrow>
+  <is_pointermap_impl bdd bddi> 
+    iteci i t e bddi 
+  <\<lambda>(pi,bddi'). is_pointermap_impl bdd' bddi' * \<up>(pi=p)>"
+proof -
+  note [simp del] = destrmi.simps lowest_topsci.simps
+    brofix.lowest_tops_impl.simps
+    brofix.restrict_top_impl.simps
+  show ?thesis
+    apply (induction arbitrary: i t e bddi bdd p bdd' rule: brofix.ite_impl.fixp_induct)
+    defer
+    apply simp
+    apply (subst iteci.simps)
+    apply (sep_auto)
+    apply (split IFEXD.split option.splits; intro impI conjI; clarsimp) []
+    apply sep_auto
+    apply sep_auto
+
+    apply (clarsimp split: Option.bind_splits)
+    apply sep_auto
+    apply (simp only: atomize_imp[symmetric] conj_imp_eq_imp_imp)
+    apply rprems
+    apply assumption
+    apply simp
+
+
+qed
+
+term brofix.ite_impl
+
+context bdd_impl begin
+thm iteci_def
+thm ite_impl.fixp_induct
+
 
 (* partial_function(option) ite_impl_opt where
 "ite_impl_opt i t e s =
